\documentclass{article}
%\usepackage{testtrino}
\usepackage{algebretta}

\begin{document}
$\pbinomio{0}{1}$
$\ptrinomio[ptinc=a^2, stinc=z]{-2}{3}{1}+ \ptrinomio{1}{-3}{2}$


$\ptrinomio{1}{-3}{1}$

$\ptrinomio{1}{0}{2}$

$\ptrinomio[ptinc=a]{-1}{3}{-1}$

$\ptrinomiop[ptinc=a, stinc=b,ttinc=c]{-2}{3}{3}$


$\ptrinomiop{1}{-3}{1}$

$\ptrinomiop{0}{0}{2}$

$\ptrinomiop[ptinc=ax^2, stinc=b]{-1}{3}{1}$

$\ptrinomio[ptinc=a^2, stinc=z]{-2}{3}{1}+ \ptrinomio{1}{-3}{2}$


$\ptrinomios{1}{-3}{1}$

$\ptrinomios{1}{0}{2}$

$\ptrinomios[ptinc=a, stinc=c]{-1}{3}{-1}$

$\ptrinomios[ptinc=a, stinc=b]{-2}{3}{3}$


$\ptrinomios{1}{-3}{1}$

$\ptrinomios{1}{0}{2}$

$\ptrinomios{-1}{0}{-2}$


$\ptrinomiop[ptinc=ax^2, stinc=b]{-1}{3}{1}$
\end{document}